Use predicate to define shift and un shifted part

Ex6.dfy
@@ -1,8 +1,94 @@
 predicate Sorted(a:array<int>, low:int, high:int) 
     reads a 
     // index must not out of bound 
-    requires 0 <=low
-    requires     high <= a.Length
+    requires 0<= low <= high  <= a.Length
 {
-    forall i :: low <= i< high-1 ==> a[i]<= a[i+1]
+    forall j,k:: 0<=j<k<high ==> a[j]<=a[k] 
+}
+
+predicate SortedExcept(a:array<int>,low:int, high:int, except:int )
+    reads a 
+    requires 0<= low <= high  <= a.Length
+    requires low <= except <= high
+{
+    forall j,k:: (0<=j<k<high && j != except && k != except) ==> a[j]<=a[k] 
+}
+
+predicate Shifted(a:array<int>, a_old:seq<int>, low:int, high:int)
+    reads a 
+    requires a.Length == |a_old|
+    requires 0<= low <= high  < a.Length
+{
+    // define of shuffle 
+    (forall i ::  (low < i <= high )==> a[i] == a_old[i-1]) && 
+    // proof both part are same 
+    a[low + 1 .. high+1] == a_old[low..high] && 
+    // proof the multiset 
+    multiset(a[low + 1 .. high+1]) == multiset(a_old[low..high])
+}
+
+predicate unShifted(a:array<int>, a_old:seq<int>, low:int, high:int)
+    reads a 
+    requires a.Length == |a_old|
+    requires 0<= low <= high  < a.Length
+{
+    // unshifted should be all the same 
+    (forall i:: (low <= i < high) ==> a[i] == a_old[i] ) &&
+    // use this for all we can show that the mulitset of these tow things are same 
+    multiset(a[0..high]) == multiset(a_old[low..high])
+}
+
+
+
+
+method InsertionSortShuffle(a: array<int>)
+
+requires a.Length>1
+ensures Sorted(a, 0, a.Length);
+ensures multiset(a[..]) == multiset(old(a[..]));
+modifies a;
+{
+    var up:=1;
+    while (up < a.Length)
+        decreases a.Length - up 
+        invariant 1 <= up <= a.Length;
+        invariant Sorted(a, 0, up);
+        invariant multiset(a[..]) == multiset(old(a[..]));
+    {
+        var injectValue := a[up];
+        var injectPoint := up;
+        ghost var  a_old := a[..];
+
+        while ( injectPoint>= 1 &&  a[injectPoint - 1] > injectValue)
+            decreases injectPoint;
+            invariant SortedExcept(a,0, up, injectPoint)
+            // defined the shift and unshifted part 
+            invariant unShifted(a, a_old, 0, injectPoint);
+            invariant Shifted(a, a_old, injectPoint, up);
+            // define of inject value 
+            invariant injectValue == a_old[up];
+            // first proof of content isn't changed 
+            invariant multiset(a[injectPoint + 1 .. up+1])+multiset({injectValue}) == multiset(a_old[injectPoint..up+1]);
+
+        {
+            a[injectPoint] := a[injectPoint -1];
+            injectPoint := injectPoint -1;
+        }
+
+        a[injectPoint] :=  injectValue;
+        up:=up+1;
+    }
+}
+method Main()
+{
+// do not change this code
+var a := new int[][6,2,0,6,3,5,0,4,1,6,0]; // testcase 1
+var msa := multiset(a[..]);
+InsertionSortShuffle(a);
+assert Sorted(a, 0, a.Length);
+var msa_post := multiset(a[..]);
+assert msa==msa_post;
+var b := new int[][8,7]; // testcase 2
+InsertionSortShuffle(b);
+print a[..], b[..];
 }
